{-# OPTIONS --without-K --rewriting #-}

open import Base

module OpetopicTypes where

  data Frm (A : 𝕌) : 𝕌
  data Tree (A : 𝕌) : (f : Frm A) → 𝕌

  postulate
  
    Cell : (A : 𝕌) (f : Frm A) → 𝕌
    Pos : {A : 𝕌} (f : Frm A) → Tree A f → 𝕌

  Typ : {A : 𝕌} (f : Frm A)
    → (σ : Tree A f) (p : Pos f σ) → Frm A
    
  Inh : {A : 𝕌} (f : Frm A)
    → (σ : Tree A f) (p : Pos f σ) → Cell A (Typ f σ p)

  infixl 30 _∥_▸_
  
  data Frm (A : 𝕌) where
    ● : Frm A
    _∥_▸_ : (f : Frm A) (σ : Tree A f) (τ : Cell A f) → Frm A 

  {-# TERMINATING #-}
  η : {A : 𝕌} (f : Frm A) → Cell A f → Tree A f

  μ : {A : 𝕌} (f : Frm A) (σ : Tree A f)
    → (κ : (p : Pos f σ) → Tree A (Typ f σ p))
    → Tree A f

  γ : {A : 𝕌} (f : Frm A)
    → (σ : Tree A f) (τ : Cell A f) (ρ : Tree A (f ∥ σ ▸ τ))
    → (ϕ : (p : Pos f σ) → Tree A (Typ f σ p))
    → (ψ : (p : Pos f σ) → Tree A (Typ f σ p ∥ ϕ p ▸ Inh f σ p))
    → Tree A (f ∥ μ f σ ϕ ▸ τ)

  η-pos : {A : 𝕌} (f : Frm A)
    → (α : Cell A f) → Pos f (η f α)

  η-pos-elim : {A : 𝕌} (f : Frm A) (α : Cell A f)
    → (X : (p : Pos f (η f α)) → 𝕌)
    → (η-pos* : X (η-pos f α))
    → (p : Pos f (η f α)) → X p

  μ-pos : {A : 𝕌} (f : Frm A) (σ : Tree A f)
    → (κ : (p : Pos f σ) → Tree A (Typ f σ p))
    → (p : Pos f σ) (q : Pos (Typ f σ p) (κ p))
    → Pos f (μ f σ κ)

  μ-pos-fst : {A : 𝕌} (f : Frm A) (σ : Tree A f)
    → (κ : (p : Pos f σ) → Tree A (Typ f σ p))
    → Pos f (μ f σ κ) → Pos f σ

  μ-pos-snd : {A : 𝕌} (f : Frm A) (σ : Tree A f)
    → (κ : (p : Pos f σ) → Tree A (Typ f σ p))
    → (p : Pos f (μ f σ κ)) → Pos (Typ f σ (μ-pos-fst f σ κ p)) (κ (μ-pos-fst f σ κ p))

  γ-pos-inl : {A : 𝕌} (f : Frm A)
    → (σ : Tree A f) (τ : Cell A f) (ρ : Tree A (f ∥ σ ▸ τ))
    → (ϕ : (p : Pos f σ) → Tree A (Typ f σ p))
    → (ψ : (p : Pos f σ) → Tree A (Typ f σ p ∥ ϕ p ▸ Inh f σ p))
    → Pos (f ∥ σ ▸ τ) ρ → Pos (f ∥ μ f σ ϕ ▸ τ) (γ f σ τ ρ ϕ ψ)

  γ-pos-inr : {A : 𝕌} (f : Frm A)
    → (σ : Tree A f) (τ : Cell A f) (ρ : Tree A (f ∥ σ ▸ τ))
    → (ϕ : (p : Pos f σ) → Tree A (Typ f σ p))
    → (ψ : (p : Pos f σ) → Tree A (Typ f σ p ∥ ϕ p ▸ Inh f σ p))
    → (p : Pos f σ) (q : Pos (Typ f σ p ∥ ϕ p ▸ Inh f σ p) (ψ p))
    → Pos (f ∥ μ f σ ϕ ▸ τ) (γ f σ τ ρ ϕ ψ)

  γ-pos-elim : {A : 𝕌} (f : Frm A)
    → (σ : Tree A f) (τ : Cell A f) (ρ : Tree A (f ∥ σ ▸ τ))
    → (ϕ : (p : Pos f σ) → Tree A (Typ f σ p))
    → (ψ : (p : Pos f σ) → Tree A (Typ f σ p ∥ ϕ p ▸ Inh f σ p))
    → (X : Pos (f ∥ μ f σ ϕ ▸ τ) (γ f σ τ ρ ϕ ψ) → 𝕌)
    → (inl* : (p : Pos (f ∥ σ ▸ τ) ρ) → X (γ-pos-inl f σ τ ρ ϕ ψ p))
    → (inr* : (p : Pos f σ) (q : Pos (Typ f σ p ∥ ϕ p ▸ Inh f σ p) (ψ p)) → X (γ-pos-inr f σ τ ρ ϕ ψ p q))
    → (p : Pos (f ∥ μ f σ ϕ ▸ τ) (γ f σ τ ρ ϕ ψ)) → X p

  data Tree (A : 𝕌) where
    ob : (α : Cell A ●) → Tree A ●
    lf : (f : Frm A) (α : Cell A f)
      → Tree A (f ∥ η f α ▸ α)
    nd : (f : Frm A) 
      → (σ : Tree A f) (τ : Cell A f)  (α : Cell A (f ∥ σ ▸ τ))
      → (δ : (p : Pos f σ) → Tree A (Typ f σ p))
      → (ε : (p : Pos f σ) → Tree A (Typ f σ p ∥ δ p ▸ Inh f σ p))
      → Tree A (f ∥ μ f σ δ ▸ τ)

  postulate

    ob-pos : {A : 𝕌} (α : Cell A ●)
      → Pos ● (ob α)

    ob-pos-elim : {A : 𝕌} (α : Cell A ●)
      → (X : Pos ● (ob α) → 𝕌)
      → (x : X (ob-pos α))
      → (p : Pos ● (ob α)) → X p

    ob-pos-elim-β : {A : 𝕌} (α : Cell A ●)
      → (X : Pos ● (ob α) → 𝕌)
      → (x : X (ob-pos α))
      → ob-pos-elim α X x (ob-pos α) ↦ x
    {-# REWRITE ob-pos-elim-β #-}

    lf-pos-elim : {A : 𝕌} (f : Frm A) (α : Cell A f)
      → (X : Pos (f ∥ η f α ▸ α) (lf f α) → 𝕌)
      → (p : Pos (f ∥ η f α ▸ α) (lf f α)) → X p

    nd-pos-here : {A : 𝕌} (f : Frm A) 
      → (σ : Tree A f) (τ : Cell A f)  (α : Cell A (f ∥ σ ▸ τ))
      → (δ : (p : Pos f σ) → Tree A (Typ f σ p))
      → (ε : (p : Pos f σ) → Tree A (Typ f σ p ∥ δ p ▸ Inh f σ p))
      → Pos (f ∥ μ f σ δ ▸ τ) (nd f σ τ α δ ε)

    nd-pos-there : {A : 𝕌} (f : Frm A) 
      → (σ : Tree A f) (τ : Cell A f)  (α : Cell A (f ∥ σ ▸ τ))
      → (δ : (p : Pos f σ) → Tree A (Typ f σ p))
      → (ε : (p : Pos f σ) → Tree A (Typ f σ p ∥ δ p ▸ Inh f σ p))
      → (p : Pos f σ) (q : Pos (Typ f σ p ∥ δ p ▸ Inh f σ p) (ε p))
      → Pos (f ∥ μ f σ δ ▸ τ) (nd f σ τ α δ ε)
      
    nd-pos-elim : {A : 𝕌} (f : Frm A) 
      → (σ : Tree A f) (τ : Cell A f)  (α : Cell A (f ∥ σ ▸ τ))
      → (δ : (p : Pos f σ) → Tree A (Typ f σ p))
      → (ε : (p : Pos f σ) → Tree A (Typ f σ p ∥ δ p ▸ Inh f σ p))
      → (X : Pos (f ∥ μ f σ δ ▸ τ) (nd f σ τ α δ ε) → 𝕌)
      → (here* : X (nd-pos-here f σ τ α δ ε))
      → (there* : (p : Pos f σ) (q : Pos (Typ f σ p ∥ δ p ▸ Inh f σ p) (ε p))
           → X (nd-pos-there f σ τ α δ ε p q))
      → (p : Pos (f ∥ μ f σ δ ▸ τ) (nd f σ τ α δ ε)) → X p

    nd-pos-elim-here-β : {A : 𝕌} (f : Frm A) 
      → (σ : Tree A f) (τ : Cell A f)  (α : Cell A (f ∥ σ ▸ τ))
      → (δ : (p : Pos f σ) → Tree A (Typ f σ p))
      → (ε : (p : Pos f σ) → Tree A (Typ f σ p ∥ δ p ▸ Inh f σ p))
      → (X : Pos (f ∥ μ f σ δ ▸ τ) (nd f σ τ α δ ε) → 𝕌)
      → (here* : X (nd-pos-here f σ τ α δ ε))
      → (there* : (p : Pos f σ) (q : Pos (Typ f σ p ∥ δ p ▸ Inh f σ p) (ε p))
           → X (nd-pos-there f σ τ α δ ε p q))
      → nd-pos-elim f σ τ α δ ε X here* there* (nd-pos-here f σ τ α δ ε) ↦ here*
    {-# REWRITE nd-pos-elim-here-β #-}

    nd-pos-elim-there-β : {A : 𝕌} (f : Frm A) 
      → (σ : Tree A f) (τ : Cell A f)  (α : Cell A (f ∥ σ ▸ τ))
      → (δ : (p : Pos f σ) → Tree A (Typ f σ p))
      → (ε : (p : Pos f σ) → Tree A (Typ f σ p ∥ δ p ▸ Inh f σ p))
      → (X : Pos (f ∥ μ f σ δ ▸ τ) (nd f σ τ α δ ε) → 𝕌)
      → (here* : X (nd-pos-here f σ τ α δ ε))
      → (there* : (p : Pos f σ) (q : Pos (Typ f σ p ∥ δ p ▸ Inh f σ p) (ε p))
           → X (nd-pos-there f σ τ α δ ε p q))
      → (p : Pos f σ) (q : Pos (Typ f σ p ∥ δ p ▸ Inh f σ p) (ε p))
      → nd-pos-elim f σ τ α δ ε X here* there* (nd-pos-there f σ τ α δ ε p q) ↦ there* p q
    {-# REWRITE nd-pos-elim-there-β #-}

  --
  --  Definining position types and inhabitants
  --

  -- Typ : {A : 𝕌} (f : Frm A)
  --   → (σ : Tree A f) (p : Pos f σ) → Frm A
  Typ _ (ob α) p = ●
  Typ _ (lf f α) = lf-pos-elim f α (λ _ → Frm _)
  Typ _ (nd f σ τ α δ ε) =
    let X p = Frm _
        th p q = Typ (Typ f σ p ∥ δ p ▸ Inh f σ p) (ε p) q
    in nd-pos-elim f σ τ α δ ε X (f ∥ σ ▸ τ) th

  -- Inh : {A : 𝕌} (f : Frm A)
  --   → (σ : Tree A f) (p : Pos f σ) → Cell A (Typ f σ p)
  Inh _ (ob α) p = α
  Inh _ (lf f α) =
    let X p = Cell _ (Typ (f ∥ η f α ▸ α) (lf f α) p)
    in lf-pos-elim f α X
  Inh _ (nd f σ τ α δ ε) =
    let X p = Cell _ (Typ (f ∥ μ f σ δ ▸ τ) (nd f σ τ α δ ε) p)
        th p q = Inh (Typ f σ p ∥ δ p ▸ Inh f σ p) (ε p) q
    in nd-pos-elim f σ τ α δ ε X α th

  postulate

    -- η-pos laws
    η-pos-typ : {A : 𝕌} (f : Frm A)
      → (α : Cell A f) (p : Pos f (η f α))
      → Typ f (η f α) p ↦ f
    {-# REWRITE η-pos-typ #-}

    η-pos-inh : {A : 𝕌} (f : Frm A)
      → (α : Cell A f) (p : Pos f (η f α))
      → Inh f (η f α) (η-pos f α) ↦ α
    {-# REWRITE η-pos-inh #-}

    η-pos-elim-β : {A : 𝕌} (f : Frm A) (α : Cell A f)
      → (X : (p : Pos f (η f α)) → 𝕌)
      → (η-pos* : X (η-pos f α))
      → η-pos-elim f α X η-pos* (η-pos f α) ↦ η-pos*
    {-# REWRITE η-pos-elim-β #-}
    
    -- μ-pos laws
    μ-pos-typ : {A : 𝕌} (f : Frm A) (σ : Tree A f)
      → (κ : (p : Pos f σ) → Tree A (Typ f σ p))
      → (p : Pos f (μ f σ κ))
      → Typ f (μ f σ κ) p ↦ Typ (Typ f σ (μ-pos-fst f σ κ p)) (κ (μ-pos-fst f σ κ p)) (μ-pos-snd f σ κ p)
    {-# REWRITE μ-pos-typ #-}

    μ-pos-inh : {A : 𝕌} (f : Frm A) (σ : Tree A f)
      → (κ : (p : Pos f σ) → Tree A (Typ f σ p))
      → (p : Pos f (μ f σ κ))
      → Inh f (μ f σ κ) p ↦ Inh (Typ f σ (μ-pos-fst f σ κ p)) (κ (μ-pos-fst f σ κ p)) (μ-pos-snd f σ κ p)
    {-# REWRITE μ-pos-inh #-}
    
    μ-pos-fst-β : {A : 𝕌} (f : Frm A) (σ : Tree A f)
      → (κ : (p : Pos f σ) → Tree A (Typ f σ p))
      → (p : Pos f σ) (q : Pos (Typ f σ p) (κ p))
      → μ-pos-fst f σ κ (μ-pos f σ κ p q) ↦ p
    {-# REWRITE μ-pos-fst-β #-}

    μ-pos-snd-β : {A : 𝕌} (f : Frm A) (σ : Tree A f)
      → (κ : (p : Pos f σ) → Tree A (Typ f σ p))
      → (p : Pos f σ) (q : Pos (Typ f σ p) (κ p))
      → μ-pos-snd f σ κ (μ-pos f σ κ p q) ↦ q
    {-# REWRITE μ-pos-snd-β #-}

    μ-pos-η : {A : 𝕌} (f : Frm A) (σ : Tree A f)
      → (κ : (p : Pos f σ) → Tree A (Typ f σ p))
      → (p : Pos f (μ f σ κ))
      → μ-pos f σ κ (μ-pos-fst f σ κ p) (μ-pos-snd f σ κ p) ↦ p
    {-# REWRITE μ-pos-η #-}

    -- μ laws
    μ-unit-r : {A : 𝕌} (f : Frm A) (σ : Tree A f) 
      → μ f σ (λ p → η (Typ f σ p) (Inh f σ p)) ↦ σ
    {-# REWRITE μ-unit-r #-}

    μ-unit-l : {A : 𝕌} (f : Frm A)
      → (α : Cell A f) (κ : (p : Pos f (η f α)) → Tree A (Typ f (η f α) p))
      → μ f (η f α) κ ↦ κ (η-pos f α)
    {-# REWRITE μ-unit-l #-}

    μ-assoc : {A : 𝕌} (f : Frm A) (σ : Tree A f)
      → (κ : (p : Pos f σ) → Tree A (Typ f σ p))
      → (θ : (p : Pos f (μ f σ κ)) → Tree A (Typ f (μ f σ κ) p))
      → μ f (μ f σ κ) θ ↦ μ f σ (λ p → μ (Typ f σ p) (κ p) (λ q → θ (μ-pos f σ κ p q)))
    {-# REWRITE μ-assoc #-}
    
    -- γ elim comp rules
    γ-pos-elim-inl-β : {A : 𝕌} (f : Frm A)
      → (σ : Tree A f) (τ : Cell A f) (ρ : Tree A (f ∥ σ ▸ τ))
      → (ϕ : (p : Pos f σ) → Tree A (Typ f σ p))
      → (ψ : (p : Pos f σ) → Tree A (Typ f σ p ∥ ϕ p ▸ Inh f σ p))
      → (X : Pos (f ∥ μ f σ ϕ ▸ τ) (γ f σ τ ρ ϕ ψ) → 𝕌)
      → (inl* : (p : Pos (f ∥ σ ▸ τ) ρ) → X (γ-pos-inl f σ τ ρ ϕ ψ p))
      → (inr* : (p : Pos f σ) (q : Pos (Typ f σ p ∥ ϕ p ▸ Inh f σ p) (ψ p)) → X (γ-pos-inr f σ τ ρ ϕ ψ p q))
      → (p : Pos (f ∥ σ ▸ τ) ρ)
      → γ-pos-elim f σ τ ρ ϕ ψ X inl* inr* (γ-pos-inl f σ τ ρ ϕ ψ p) ↦ inl* p
    {-# REWRITE γ-pos-elim-inl-β #-}

    γ-pos-elim-inr-β : {A : 𝕌} (f : Frm A)
      → (σ : Tree A f) (τ : Cell A f) (ρ : Tree A (f ∥ σ ▸ τ))
      → (ϕ : (p : Pos f σ) → Tree A (Typ f σ p))
      → (ψ : (p : Pos f σ) → Tree A (Typ f σ p ∥ ϕ p ▸ Inh f σ p))
      → (X : Pos (f ∥ μ f σ ϕ ▸ τ) (γ f σ τ ρ ϕ ψ) → 𝕌)
      → (inl* : (p : Pos (f ∥ σ ▸ τ) ρ) → X (γ-pos-inl f σ τ ρ ϕ ψ p))
      → (inr* : (p : Pos f σ) (q : Pos (Typ f σ p ∥ ϕ p ▸ Inh f σ p) (ψ p)) → X (γ-pos-inr f σ τ ρ ϕ ψ p q))
      → (p : Pos f σ) (q : Pos (Typ f σ p ∥ ϕ p ▸ Inh f σ p) (ψ p))
      → γ-pos-elim f σ τ ρ ϕ ψ X inl* inr* (γ-pos-inr f σ τ ρ ϕ ψ p q) ↦ inr* p q
    {-# REWRITE γ-pos-elim-inr-β #-}
    
    -- γ pos laws
    γ-pos-typ : {A : 𝕌} (f : Frm A)
      → (σ : Tree A f) (τ : Cell A f) (ρ : Tree A (f ∥ σ ▸ τ))
      → (ϕ : (p : Pos f σ) → Tree A (Typ f σ p))
      → (ψ : (p : Pos f σ) → Tree A (Typ f σ p ∥ ϕ p ▸ Inh f σ p))
      → (p : Pos (f ∥ μ f σ ϕ ▸ τ) (γ f σ τ ρ ϕ ψ))
      → Typ (f ∥ μ f σ ϕ ▸ τ) (γ f σ τ ρ ϕ ψ) p ↦
          γ-pos-elim f σ τ ρ ϕ ψ (λ _ → Frm A)
                     (λ p → Typ (f ∥ σ ▸ τ) ρ p)
                     (λ p q → Typ (Typ f σ p ∥ ϕ p ▸ Inh f σ p) (ψ p) q) p
    {-# REWRITE γ-pos-typ #-}

    γ-pos-inh : {A : 𝕌} (f : Frm A)
      → (σ : Tree A f) (τ : Cell A f) (ρ : Tree A (f ∥ σ ▸ τ))
      → (ϕ : (p : Pos f σ) → Tree A (Typ f σ p))
      → (ψ : (p : Pos f σ) → Tree A (Typ f σ p ∥ ϕ p ▸ Inh f σ p))
      → (p : Pos (f ∥ μ f σ ϕ ▸ τ) (γ f σ τ ρ ϕ ψ))
      → Inh (f ∥ μ f σ ϕ ▸ τ) (γ f σ τ ρ ϕ ψ) p ↦
          γ-pos-elim f σ τ ρ ϕ ψ (λ p → Cell A (Typ (f ∥ μ f σ ϕ ▸ τ) (γ f σ τ ρ ϕ ψ) p))
            (λ p → Inh (f ∥ σ ▸ τ) ρ p)
            (λ p q → Inh (Typ f σ p ∥ ϕ p ▸ Inh f σ p) (ψ p) q) p
    {-# REWRITE γ-pos-inh #-}

    -- γ laws
    γ-unit-r : {A : 𝕌} (f : Frm A)
      → (σ : Tree A f) (τ : Cell A f) (ρ : Tree A (f ∥ σ ▸ τ))
      → γ f σ τ ρ (λ p → η (Typ f σ p) (Inh f σ p)) (λ p → lf (Typ f σ p) (Inh f σ p)) ↦ ρ
    {-# REWRITE γ-unit-r #-}

    -- Doesn't seem to be necessary for typechecking below, but ...
    γ-assoc : {A : 𝕌} (f : Frm A)
      → (σ : Tree A f) (τ : Cell A f) (ρ : Tree A (f ∥ σ ▸ τ))
      → (ϕ₀ : (p : Pos f σ) → Tree A (Typ f σ p))
      → (ψ₀ : (p : Pos f σ) → Tree A (Typ f σ p ∥ ϕ₀ p ▸ Inh f σ p))
      → (ϕ₁ : (p : Pos f (μ f σ ϕ₀)) → Tree A (Typ f (μ f σ ϕ₀) p))
      → (ψ₁ : (p : Pos f (μ f σ ϕ₀)) → Tree A (Typ f (μ f σ ϕ₀) p ∥ ϕ₁ p ▸ Inh f (μ f σ ϕ₀) p))
      → γ f (μ f σ ϕ₀) τ (γ f σ τ ρ ϕ₀ ψ₀) ϕ₁ ψ₁ ↦
        γ f σ τ ρ (λ p → μ (Typ f σ p) (ϕ₀ p) (λ q → ϕ₁ (μ-pos f σ ϕ₀ p q)))
                (λ p → γ (Typ f σ p) (ϕ₀ p) (Inh f σ p) (ψ₀ p)
                         (λ q → ϕ₁ (μ-pos f σ ϕ₀ p q))
                         (λ q → ψ₁ (μ-pos f σ ϕ₀ p q)))

    -- Finally, it seems there should be the interchange law
    -- Is this sufficient?
    γμ-ichg : {A : 𝕌} (f : Frm A)
      → (σ : Tree A f) (τ : Cell A f) (ρ : Tree A (f ∥ σ ▸ τ))
      → (ϕ : (p : Pos f σ) → Tree A (Typ f σ p))
      → (ψ : (p : Pos f σ) → Tree A (Typ f σ p ∥ ϕ p ▸ Inh f σ p))
      → (κ : (p : Pos (f ∥ σ ▸ τ) ρ) → Tree A (Typ (f ∥ σ ▸ τ) ρ p))
      → γ f σ τ (μ (f ∥ σ ▸ τ) ρ κ) ϕ ψ ↦
        μ (f ∥ μ f σ ϕ ▸ τ) (γ f σ τ ρ ϕ ψ)
          (γ-pos-elim f σ τ ρ ϕ ψ
            (λ p → Tree A (Typ (f ∥ μ f σ ϕ ▸ τ) (γ f σ τ ρ ϕ ψ) p)) κ
            (λ p q → η ((Typ (Typ f σ p ∥ ϕ p ▸ Inh f σ p) (ψ p) q)) (Inh (Typ f σ p ∥ ϕ p ▸ Inh f σ p) (ψ p) q)))

  -- η : {A : 𝕌} (f : Frm A) → Cell A f → Tree A f
  η ● α = ob α
  η (f ∥ σ ▸ τ) α =  
    let η-dec p = η (Typ f σ p) (Inh f σ p)
        lf-dec p = lf (Typ f σ p) (Inh f σ p)
    in nd f σ τ α η-dec lf-dec

  -- η-pos : {A : 𝕌} (f : Frm A)
  --   → (α : Cell A f) → Pos f (η f α)
  η-pos ● α = ob-pos α
  η-pos (f ∥ σ ▸ τ) α =
    let η-dec p = η (Typ f σ p) (Inh f σ p)
        lf-dec p = lf (Typ f σ p) (Inh f σ p)
    in nd-pos-here f σ τ α η-dec lf-dec

  -- η-pos-elim : {A : 𝕌} (f : Frm A) (α : Cell A f)
  --   → (X : (p : Pos f (η f α)) → 𝕌)
  --   → (η-pos* : X (η-pos α))
  --   → (p : Pos f (η f α)) → X p
  η-pos-elim ● α X η-pos* p =
    ob-pos-elim α (λ p → X (ob-pos α) → X p)
      (λ p → p) p η-pos* 
  η-pos-elim (f ∥ σ ▸ τ) α X η-pos* p =
    let η-dec p = η (Typ f σ p) (Inh f σ p)
        lf-dec p = lf (Typ f σ p) (Inh f σ p)
    in nd-pos-elim f σ τ α η-dec lf-dec (λ p → X (nd-pos-here f σ τ α η-dec lf-dec) → X p)
         (λ x → x) (λ p q → lf-pos-elim (Typ f σ p) (Inh f σ p)
                            (λ q → X (nd-pos-here f σ τ α η-dec lf-dec)
                                 → X (nd-pos-there f σ τ α η-dec lf-dec p q)) q) p η-pos*

  -- μ : {A : 𝕌} (f : Frm A) (σ : Tree A f)
  --   → (κ : (p : Pos f σ) → Tree A (Typ f σ p))
  --   → Tree A f
  μ .● (ob α) κ = κ (ob-pos α)
  μ .(f ∥ (η f α) ▸ α) (lf f α) κ = lf f α
  μ .(f ∥ (μ f σ δ) ▸ τ) (nd f σ τ α δ ε) κ = 
    let w = κ (nd-pos-here f σ τ α δ ε)
        κ' p q = κ (nd-pos-there f σ τ α δ ε p q)
        ψ p = μ (Typ f σ p ∥ δ p ▸ Inh f σ p) (ε p) (κ' p)
    in γ f σ τ w δ ψ


  -- γ : {A : 𝕌} (f : Frm A)
  --   → (σ : Tree A f) (τ : Cell A f) (ρ : Tree A (f ∥ σ ▸ τ))
  --   → (ϕ : (p : Pos f σ) → Tree A (Typ f σ p))
  --   → (ψ : (p : Pos f σ) → Tree A (Typ f σ p ∥ ϕ p ▸ Inh f σ p))
  --   → Tree A (f ∥ μ f σ ϕ ▸ τ)
  γ .f .(η f τ) .τ (lf f τ) ϕ ψ = ψ (η-pos f τ)
  γ .f .(μ f σ δ) .τ (nd f σ τ α δ ε) ϕ ψ =
    let ϕ' p q = ϕ (μ-pos f σ δ p q)
        ψ' p q = ψ (μ-pos f σ δ p q)
        δ' p = μ (Typ f σ p) (δ p) (ϕ' p)
        ε' p = γ (Typ f σ p) (δ p) (Inh f σ p) (ε p) (ϕ' p) (ψ' p)
    in nd f σ τ α δ' ε'

  -- μ-pos : {A : 𝕌} (f : Frm A) (σ : Tree A f)
  --   → (κ : (p : Pos f σ) → Tree A (Typ f σ p))
  --   → (p : Pos f σ) (q : Pos (Typ f σ p) (κ p))
  --   → Pos f (μ f σ κ)
  μ-pos _ (ob α) κ p q =
    let X p = Pos ● (κ p) → Pos ● (κ (ob-pos α))
    in ob-pos-elim α X (λ q → q) p q  -- would be trivial given η for ob-pos
  μ-pos _ (lf f α) κ p q =
    let X _ = Pos (f ∥ η f α ▸ α) (lf f α)
    in lf-pos-elim f α X p 
  μ-pos _ (nd f σ τ α δ ε) κ =
    let X p = Pos (Typ (f ∥ μ f σ δ ▸ τ) (nd f σ τ α δ ε) p) (κ p)
              → Pos (f ∥ μ f σ δ ▸ τ) (μ (f ∥ μ f σ δ ▸ τ) (nd f σ τ α δ ε) κ)
        w = κ (nd-pos-here f σ τ α δ ε)
        κ' p q = κ (nd-pos-there f σ τ α δ ε p q)
        ψ p = μ (Typ f σ p ∥ δ p ▸ Inh f σ p) (ε p) (κ' p)
    in nd-pos-elim f σ τ α δ ε X (γ-pos-inl f σ τ w δ ψ) 
         (λ p q r → γ-pos-inr f σ τ w δ ψ p
           (μ-pos (Typ f σ p ∥ δ p ▸ Inh f σ p) (ε p) (κ' p) q r))


  -- μ-pos-fst : {A : 𝕌} (f : Frm A) (σ : Tree A f)
  --   → (κ : (p : Pos f σ) → Tree A (Typ f σ p))
  --   → Pos f (μ f σ κ) → Pos f σ
  μ-pos-fst .● (ob α) κ p = ob-pos α
  μ-pos-fst .(f ∥ η f α ▸ α) (lf f α) κ p = p
  μ-pos-fst .(f ∥ μ f σ δ ▸ τ) (nd f σ τ α δ ε) κ = 
    let w = κ (nd-pos-here f σ τ α δ ε)
        κ' p q = κ (nd-pos-there f σ τ α δ ε p q)
        ψ p = μ (Typ f σ p ∥ δ p ▸ Inh f σ p) (ε p) (κ' p)
    in γ-pos-elim f σ τ w δ ψ _
         (λ _ → nd-pos-here f σ τ α δ ε)
         (λ p q → nd-pos-there f σ τ α δ ε p
                    (μ-pos-fst (Typ f σ p ∥ δ p ▸ Inh f σ p) (ε p) (κ' p) q))

  -- μ-pos-snd : {A : 𝕌} (f : Frm A) (σ : Tree A f)
  --   → (κ : (p : Pos f σ) → Tree A (Typ f σ p))
  --   → (p : Pos f (μ f σ κ)) → Pos (κ (μ-pos-fst f σ κ p))
  μ-pos-snd .● (ob α) κ p = p
  μ-pos-snd .(f ∥ η f α ▸ α) (lf f α) κ = lf-pos-elim f α _ 
  μ-pos-snd .(f ∥ μ f σ δ ▸ τ) (nd f σ τ α δ ε) κ = 
    let w = κ (nd-pos-here f σ τ α δ ε)
        κ' p q = κ (nd-pos-there f σ τ α δ ε p q)
        ψ p = μ (Typ f σ p ∥ δ p ▸ Inh f σ p) (ε p) (κ' p)
    in γ-pos-elim f σ τ w δ ψ _
         (λ p → p)
         (λ p q → μ-pos-snd (Typ f σ p ∥ δ p ▸ Inh f σ p) (ε p) (κ' p) q)

  -- γ-pos-inl : {A : 𝕌} (f : Frm A)
  --   → (σ : Tree A f) (τ : Cell A f) (ρ : Tree A (f ∥ σ ▸ τ))
  --   → (ϕ : (p : Pos f σ) → Tree A (Typ f σ p))
  --   → (ψ : (p : Pos f σ) → Tree A (Typ f σ p ∥ ϕ p ▸ Inh f σ p))
  --   → Pos (f ∥ σ ▸ τ) ρ → Pos (f ∥ μ f σ ϕ ▸ τ) (γ f σ τ ρ ϕ ψ)
  γ-pos-inl .f .(η f α) .α (lf f α) ϕ ψ = lf-pos-elim f α _
  γ-pos-inl .f .(μ f σ δ) .τ (nd f σ τ α δ ε) ϕ ψ = 
    let ϕ' p q = ϕ (μ-pos f σ δ p q)
        ψ' p q = ψ (μ-pos f σ δ p q)
        δ' p = μ (Typ f σ p) (δ p) (ϕ' p)
        ε' p = γ (Typ f σ p) (δ p) (Inh f σ p) (ε p) (ϕ' p) (ψ' p)
    in nd-pos-elim f σ τ α δ ε _
         (nd-pos-here f σ τ α δ' ε')
         (λ p q → nd-pos-there f σ τ α δ' ε' p
                    (γ-pos-inl (Typ f σ p) (δ p) (Inh f σ p) (ε p) (ϕ' p) (ψ' p) q))

  -- γ-pos-inr : {A : 𝕌} (f : Frm A)
  --   → (σ : Tree A f) (τ : Cell A f) (ρ : Tree A (f ∥ σ ▸ τ))
  --   → (ϕ : (p : Pos f σ) → Tree A (Typ f σ p))
  --   → (ψ : (p : Pos f σ) → Tree A (Typ f σ p ∥ ϕ p ▸ Inh f σ p))
  --   → (p : Pos f σ) (q : Pos (ψ p))
  --   → Pos (f ∥ μ f σ ϕ ▸ τ) (γ f σ τ ρ ϕ ψ)
  γ-pos-inr .f .(η f α) .α (lf f α) ϕ ψ p q =
    η-pos-elim f α (λ p → Pos (f ∥ ϕ p ▸ Inh f (η f α) p) (ψ p) → Pos (f ∥ ϕ (η-pos f α) ▸ α) (ψ (η-pos f α)))
      (λ p → p) p q
  γ-pos-inr .f .(μ f σ δ) .τ (nd f σ τ α δ ε) ϕ ψ p q = 
    let ϕ' p q = ϕ (μ-pos f σ δ p q)
        ψ' p q = ψ (μ-pos f σ δ p q)
        δ' p = μ (Typ f σ p) (δ p) (ϕ' p)
        ε' p = γ (Typ f σ p) (δ p) (Inh f σ p) (ε p) (ϕ' p) (ψ' p)
        p₀ = μ-pos-fst f σ δ p
        p₁ = μ-pos-snd f σ δ p
    in nd-pos-there f σ τ α δ' ε' p₀
         (γ-pos-inr (Typ f σ p₀) (δ p₀) (Inh f σ p₀) (ε p₀) (ϕ' p₀) (ψ' p₀) p₁ q)

  -- γ-pos-elim : {A : 𝕌} (f : Frm A)
  --   → (σ : Tree A f) (τ : Cell A f) (ρ : Tree A (f ∥ σ ▸ τ))
  --   → (ϕ : (p : Pos f σ) → Tree A (Typ f σ p))
  --   → (ψ : (p : Pos f σ) → Tree A (Typ f σ p ∥ ϕ p ▸ Inh f σ p))
  --   → (X : Pos (f ∥ μ f σ ϕ ▸ τ) (γ f σ τ ρ ϕ ψ) → 𝕌)
  --   → (inl* : (p : Pos (f ∥ σ ▸ τ) ρ) → X (γ-pos-inl f σ τ ρ ϕ ψ p))
  --   → (inr* : (p : Pos f σ) (q : Pos (ψ p)) → X (γ-pos-inr f σ τ ρ ϕ ψ p q))
  --   → (p : Pos (f ∥ μ f σ ϕ ▸ τ) (γ f σ τ ρ ϕ ψ)) → X p
  γ-pos-elim .f .(η f α) .α (lf f α) ϕ ψ X inl* inr* p = inr* (η-pos f α) p
  γ-pos-elim .f .(μ f σ δ) .τ (nd f σ τ α δ ε) ϕ ψ X inl* inr* =
    let ϕ' p q = ϕ (μ-pos f σ δ p q)
        ψ' p q = ψ (μ-pos f σ δ p q)
        δ' p = μ (Typ f σ p) (δ p) (ϕ' p)
        ε' p = γ (Typ f σ p) (δ p) (Inh f σ p) (ε p) (ϕ' p) (ψ' p)
    in nd-pos-elim f σ τ α δ' ε' X (inl* (nd-pos-here f σ τ α δ ε))
         (λ p → γ-pos-elim (Typ f σ p) (δ p) (Inh f σ p) (ε p) (ϕ' p) (ψ' p)
                  (λ q → X (nd-pos-there f σ τ α δ' ε' p q))
                  (λ q → inl* (nd-pos-there f σ τ α δ ε p q))
                  (λ q r → inr* (μ-pos f σ δ p q) r))

  --
  --  Opetopic Introduction and Elimination
  --
  
  postulate

    comp : {A : 𝕌} (f : Frm A) → Tree A f → Cell A f
    fill : {A : 𝕌} (f : Frm A) (σ : Tree A f) → Cell A (f ∥ σ ▸ comp f σ)

    J : {A : 𝕌} (f : Frm A) (σ : Tree A f)
      → (P : (τ : Cell A f) (ρ : Cell A (f ∥ σ ▸ τ)) → 𝕌)
      → (d : P (comp f σ) (fill f σ))
      → (τ : Cell A f) (ρ : Cell A (f ∥ σ ▸ τ)) → P τ ρ

    J-β : {A : 𝕌} (f : Frm A) (σ : Tree A f)
      → (P : (τ : Cell A f) (ρ : Cell A (f ∥ σ ▸ τ)) → 𝕌)
      → (d : P (comp f σ) (fill f σ))
      → J f σ P d (comp f σ) (fill f σ) ↦ d
    {-# REWRITE J-β #-}

    Cell-●-β : (A : 𝕌)
      → Cell A ● ↦ A
    {-# REWRITE Cell-●-β #-}

    -- We'll need some kind of shifting operation.  But I don't
    -- know if these need to be definitional or not ...
    frm-concat : {A : 𝕌} (f : Frm A) (g : Frm (Cell A f)) → Frm A
    Cell-concat : {A : 𝕌} (f : Frm A) (g : Frm (Cell A f))
      → Cell (Cell A f) g → Cell A (frm-concat f g)

    -- How trees work is a bit of a mystery ....
    -- tree-frm : {A : 𝕌} (f : Frm A) (g : Frm (Tree A f)) → {!!}
    -- Tree-concat : {A : 𝕌} (f : Frm A) (g : Frm (Tree A f))
    --   → Cell (Tree A f) g → {!!}
